theories/Iris/Model.v
@@ -311,16 +311,16 @@ Module Type IrisParameters
   Parameter Inline memGS : gFunctors -> Set.
   Parameter memΣ : gFunctors.
   Parameter memΣ_GpreS : forall {Σ}, subG memΣ Σ -> memGpreS Σ.
-  Parameter mem_inv : forall {Σ}, memGS Σ -> Memory -> iProp Σ.
-  Parameter mem_res : forall {Σ}, memGS Σ -> Memory -> iProp Σ.
+  Parameter mem_inv : forall `{mG : memGS Σ}, Memory -> iProp Σ.
+  Parameter mem_res : forall `{mG : memGS Σ}, Memory -> iProp Σ.
 
     (* Definition mem_inv `{sailG Σ} (μ : Z -> option Z) : iProp Σ := *)
     (*   (∃ memmap, gen_heap_ctx memmap ∗ *)
     (*      ⌜ map_Forall (fun (a : Z) v => μ a = Some v) memmap ⌝ *)
     (*   )%I. *)
 
-  Parameter mem_inv_init : forall Σ (μ : Memory), memGpreS Σ ->
-                                         ⊢ |==> ∃ mG : memGS Σ, (mem_inv mG μ ∗ mem_res mG μ)%I.
+  Parameter mem_inv_init : forall `{mGS : memGpreS Σ} (μ : Memory),
+                                         ⊢ |==> ∃ mG : memGS Σ, (mem_inv (mG := mG) μ ∗ mem_res (mG := mG) μ)%I.
 End IrisParameters.
 
 Module Type IrisResources
@@ -362,7 +362,7 @@ Module Type IrisResources
 
   #[export] Instance sailGS_irisGS {Γ τ} `{sailGS Σ} : irisGS (microsail_lang Γ τ) Σ := {
     iris_invGS := sailGS_invGS;
-    state_interp σ ns κs nt := (regs_inv σ.1 ∗ mem_inv sailGS_memGS σ.2)%I;
+    state_interp σ ns κs nt := (regs_inv σ.1 ∗ mem_inv σ.2)%I;
     fork_post _ := True%I; (* no threads forked in sail, so this is fine *)
     num_laters_per_step _ := 0;
     state_interp_mono _ _ _ _ := fupd_intro _ _;
@@ -805,12 +805,12 @@ Module Type IrisResources
 
     Lemma semWP_foreign {Γ Δ τ} {f : 𝑭𝑿 Δ τ} {es : NamedEnv (Exp Γ) Δ} {Q δ} :
       ⊢ (∀ γ μ,
-            (regs_inv γ ∗ mem_inv sailGS_memGS μ)
+            (regs_inv γ ∗ mem_inv μ)
             ={⊤,∅}=∗
         (∀ res γ' μ' ,
           ⌜ ForeignCall f (evals es δ) res γ γ' μ μ' ⌝
            ={∅}▷=∗
-           |={∅,⊤}=> (regs_inv γ' ∗ mem_inv sailGS_memGS μ') ∗
+           |={∅,⊤}=> (regs_inv γ' ∗ mem_inv μ') ∗
                       semWP (match res with inr v => stm_val _ v
                                        | inl s => stm_fail _ s
                              end) Q δ)) -∗
